basis/fsioProgConstantsScript.sml
@@ -1,0 +1,142 @@
+open preamble
+     ml_translatorTheory ml_translatorLib ml_progLib
+     cfTacticsBaseLib cfTacticsLib basisFunctionsLib
+     mlstringTheory mlcommandLineProgTheory fsFFITheory fsFFIProofTheory
+
+val _ = new_theory"fsioProgConstants";
+(* filesystem constants and corresponding hprops *)
+val _ = translation_extends "mlcommandLineProg";
+val _ = ml_prog_update (open_module "IO");
+
+val _ = process_topdecs `
+  exception BadFileName;
+  exception InvalidFD;
+  exception EndOfFile
+` |> append_prog
+
+(* 257 w8 array *)
+val iobuff_e = ``(App Aw8alloc [Lit (IntLit 257); Lit (Word8 0w)])``
+val _ = ml_prog_update
+          (add_Dlet (derive_eval_thm "iobuff_loc" iobuff_e) "iobuff" [])
+val iobuff_loc_def = definition "iobuff_loc_def"
+val iobuff_loc = EVAL``iobuff_loc`` |> curry save_thm "iobuff_loc"
+
+val _ = export_rewrites["iobuff_loc"]
+
+val IOFS_iobuff_def = Define`
+  IOFS_iobuff =
+    SEP_EXISTS v. W8ARRAY iobuff_loc v * cond (LENGTH v = 258) `;
+
+val IOFS_def = Define `
+  IOFS fs = IOx fs_ffi_part fs * IOFS_iobuff * &(wfFS fs ∧ liveFS fs)`
+
+
+val BadFileName_exn_def = Define `
+  BadFileName_exn v =
+    (v = Conv (SOME ("BadFileName", TypeExn (Long "IO" (Short "BadFileName")))) [])`
+
+val InvalidFD_exn_def = Define `
+  InvalidFD_exn v =
+    (v = Conv (SOME ("InvalidFD", TypeExn (Long "IO" (Short "InvalidFD")))) [])`
+
+val EndOfFile_exn_def = Define `
+  EndOfFile_exn v =
+    (v = Conv (SOME ("EndOfFile", TypeExn (Long "IO" (Short "EndOfFile")))) [])`
+
+val FILENAME_def = Define `
+  FILENAME s sv =
+    (STRING_TYPE s sv ∧
+     ¬MEM (CHR 0) (explode s) ∧
+     strlen s < 256)
+`;
+
+(* "end-user" property *)
+(* states that the current file system is equal to fs, except that:
+* - standard streams are opened on their usual fds with usual offsets
+*   and their content is specified by inp out and err
+* - read is the part of stdin already read, and inp is what remains 
+* - the other file descriptors and the llist are unspecified *)
+
+val STDIO_def = Define`
+ STDIO fs inp out err = SEP_EXISTS fs'. IOFS fs' *
+   &((∀ fname. ¬(fname ∈ {strlit "stdin"; strlit "stdout"; strlit "stderr"}) ⇒ 
+          ALOOKUP fs.files fname = ALOOKUP fs'.files fname) ∧
+     (ALOOKUP fs'.infds 0 = SOME (strlit "stdin", LENGTH (FST inp)) ∧
+      ALOOKUP fs'.files (strlit "stdin") = SOME (FST inp ++ SND inp)) ∧ 
+     (ALOOKUP fs'.infds 1 = SOME (strlit "stdout", LENGTH out) ∧
+      ALOOKUP fs'.files (strlit "stdout") = SOME out) ∧ 
+     (ALOOKUP fs'.infds 2 = SOME (strlit "stderr", LENGTH err) ∧
+      ALOOKUP fs'.files (strlit "stderr") = SOME err))`
+
+open cfLetAutoTheory cfLetAutoLib
+
+val UNIQUE_IOFS = Q.store_thm("UNIQUE_IOFS",
+`!s. VALID_HEAP s ==> !fs1 fs2 H1 H2. (IOFS fs1 * H1) s /\
+                                      (IOFS fs2 * H2) s ==> fs1 = fs2`,
+  rw[IOFS_def,cfHeapsBaseTheory.IOx_def, fs_ffi_part_def,
+     GSYM STAR_ASSOC,encode_def] >>
+  IMP_RES_TAC FRAME_UNIQUE_IO >> 
+  fs[encode_files_11,encode_fds_11,IO_fs_component_equality]);
+
+val IOFS_FFI_part_hprop = Q.store_thm("IOFS_FFI_part_hprop",
+  `FFI_part_hprop (IOFS fs)`,
+  rw [IOFS_def,
+      cfHeapsBaseTheory.IO_def, cfHeapsBaseTheory.IOx_def,
+      fs_ffi_part_def, cfMainTheory.FFI_part_hprop_def,
+    set_sepTheory.SEP_CLAUSES,set_sepTheory.SEP_EXISTS_THM,
+    cfHeapsBaseTheory.W8ARRAY_def,IOFS_iobuff_def,
+    cfHeapsBaseTheory.cell_def]
+  \\ fs[set_sepTheory.one_STAR,STAR_def]
+  \\ imp_res_tac SPLIT_SUBSET >> fs[SUBSET_DEF]
+  \\ metis_tac[]);
+
+val IOFS_iobuff_HPROP_INJ = Q.store_thm("IOFS_iobuff_HPROP_INJ[hprop_inj]",
+`!fs1 fs2. HPROP_INJ (IOFS fs1) (IOFS fs2) (fs2 = fs1)`,
+  rw[HPROP_INJ_def, IOFS_def, GSYM STAR_ASSOC, SEP_CLAUSES, SEP_EXISTS_THM,
+     HCOND_EXTRACT] >>
+  fs[IOFS_def,cfHeapsBaseTheory.IOx_def, fs_ffi_part_def] >>
+  EQ_TAC >> rpt DISCH_TAC >> IMP_RES_TAC FRAME_UNIQUE_IO >> fs[]);
+
+val filename_tac = metis_tac[FILENAME_def,EqualityType_NUM_BOOL,EqualityType_def];
+
+val FILENAME_UNICITY_R = Q.store_thm("FILENAME_UNICITY_R[xlet_auto_match]",
+`!f fv fv'. FILENAME f fv ==> (FILENAME f fv' <=> fv' = fv)`, filename_tac);
+
+val FILENAME_UNICITY_L = Q.store_thm("FILENAME_UNICITY_L[xlet_auto_match]",
+`!f f' fv. FILENAME f fv ==> (FILENAME f' fv <=> f' = f)`, filename_tac);
+
+val FILENAME_STRING_UNICITY_R =
+  Q.store_thm("FILENAME_STRING_UNICITY_R[xlet_auto_match]",
+  `!f fv fv'. FILENAME f fv ==> (STRING_TYPE f fv' <=> fv' = fv)`,
+  filename_tac);
+
+val FILENAME_STRING_UNICITY_L =
+  Q.store_thm("FILENAME_STRING_UNICITY_L[xlet_auto_match]",
+  `!f f' fv. FILENAME f fv ==> (STRING_TYPE f' fv <=> f' = f)`, filename_tac);
+
+val STRING_FILENAME_UNICITY_R =
+  Q.store_thm("STRING_FILENAME_UNICITY_R[xlet_auto_match]",
+  `!f fv fv'. STRING_TYPE f fv ==> 
+    (FILENAME f fv' <=> fv' = fv /\ ¬MEM #"\^@" (explode f) /\ strlen f < 256)`,
+  filename_tac);
+
+val STRING_FILENAME_UNICITY_L =
+  Q.store_thm("STRING_FILENAME_UNICITY_L[xlet_auto_match]",
+  `!f f' fv. STRING_TYPE f fv ==>
+    (FILENAME f' fv <=> f' = f /\ ¬MEM #"\^@" (explode f) /\ strlen f < 256)`, 
+  filename_tac);
+  
+val BadFileName_UNICITY = Q.store_thm("BadFileName_UNICITY[xlet_auto_match]",
+`!v1 v2. BadFileName_exn v1 ==> (BadFileName_exn v2 <=> v2 = v1)`,
+  fs[BadFileName_exn_def]);
+  
+val InvalidFD_UNICITY = Q.store_thm("InvalidFD_UNICITY[xlet_auto_match]",
+`!v1 v2. InvalidFD_exn v1 ==> (InvalidFD_exn v2 <=> v2 = v1)`,
+  fs[InvalidFD_exn_def]);
+
+val EndOfFile_UNICITY = Q.store_thm("EndOfFile_UNICITY[xlet_auto_match]",
+`!v1 v2. EndOfFile_exn v1 ==> (EndOfFile_exn v2 <=> v2 = v1)`,
+  fs[EndOfFile_exn_def]);
+
+val _ = export_theory();
+
